fairness/examples/ticketlock/fair_lock.v
@@ -7,52 +7,63 @@ From trillium.fairness.ext_models Require Import ext_models.
 
 
 Section FairLock.
-  Context `{EM: ExtModel m}. 
+  Context {M: FairModel}.
+  
+  Context {allows_unlock: fmstate M -> fmstate M -> Prop}
+          {allows_lock: fmrole M -> fmstate M -> fmstate M -> Prop}.
+  
+  (* Context {AU_DEC: forall st, Decision (∃ st', allows_unlock st st')} *)
+  (*         {AL_DEC: forall st ρ, Decision (∃ st', allows_lock ρ st st')}.  *)
 
-  Let St := fmstate m.
-  Let R := fmrole m.
-  Let EFM := @ext_model_FM _ EM. 
+  Inductive fl_EI := flU | flL (ρ: fmrole M).
+
+  Global Instance fl_EI_dec: EqDecision fl_EI. 
+  Proof using. solve_decision. Qed. 
+
+  Global Instance fl_EI_cnt: Countable fl_EI. 
+  Proof using.
+    assert (Countable (fmrole M)) as CNTρ by apply _.    
+    eapply inj_countable' with 
+      (f := fun ι => match ι with | flU => 0 | flL ρ => S (encode_nat ρ) end)
+      (g := fun n => match n with 
+                  | 0 => flU 
+                  | S n' => match decode_nat n' with
+                           | Some ρ => flL ρ
+                           | None => flU
+                           end end).
+    intros. destruct x; auto. by rewrite decode_encode_nat. 
+  Qed.
+
+  Context (fl_active_exts: fmstate M -> gset fl_EI). 
+
+  Definition fl_ETs (ι: fl_EI) :=
+    match ι with
+    | flU => allows_unlock
+    | flL ρ => allows_lock ρ
+    end.
+
+  Context (fl_active_exts_spec: 
+            forall st ι, ι ∈ fl_active_exts st <-> ∃ st', fl_ETs ι st st'). 
+
+  (* Context {EM: ExtModel M}. *)
+  Definition FL_EM: ExtModel M.
+    refine {| active_exts_spec := fl_active_exts_spec |}.
+  Defined. 
+
+  Let St := fmstate M.
+  Let R := fmrole M.
+  Let EFM := @ext_model_FM _ FL_EM. 
 
   Context (can_lock_st can_unlock_st has_lock_st active_st: R -> St -> Prop).
   Context {active_st_Dec: forall ρ st, Decision (active_st ρ st)}. 
-  Context (is_init_st: St -> Prop). 
+  (* Context (is_init_st: St -> Prop). *)
+  Context (state_wf: St -> Prop). 
   
-
-  (* Definition eventual_release (tr: mtrace EFM) (ρ: R) (i: nat) := *)
-  (*   forall (ρ': R) j st' (JTH: tr S!! j = Some st') *)
-  (*     (HAS_LOCK: has_lock_st ρ' st') *)
-  (*     (PREVr: ρ' = ρ -> j < i), *)
-  (*   exists k st'', tr S!! k = Some st'' /\ j <= k /\ active_st ρ' st''. *)
-  (* Definition eventual_release (tr: mtrace EFM) (ρ: R) (i: nat) := *)
-  (*   forall (ρ': R) j st' (JTH: tr S!! j = Some st') *)
-  (*     (HAS_LOCK: has_lock_st ρ' st'), *)
-  (*   exists k st'', tr S!! k = Some st'' /\ j <= k /\ active_st ρ' st''. *)
   Definition eventual_release (tr: mtrace EFM) (ρ: R) (i: nat) :=
     forall (ρ': R) j st' (JTH: tr S!! j = Some st')
       (HAS_LOCK: has_lock_st ρ' st')
       (AFTER: i <= j -> (ρ' ≠ ρ /\ forall k st_k (BETWEEN: i <= k <= j) (KTH: tr S!! k = Some st_k), ¬ has_lock_st ρ st_k)),
       exists k st'', tr S!! k = Some st'' /\ j <= k /\ active_st ρ' st''.
-
-  (* Lemma eventual_release_strenghten tr ρ i *)
-  (*   (EV_REL: eventual_release tr ρ i): *)
-  (*   forall ρ' j st' (JTH: tr S!! j = Some st') *)
-  (*     (HAS_LOCK: has_lock_st ρ' st') *)
-  (*     (PREVr: ρ' = ρ -> j < i), *)
-  (*   exists k, ClassicalFacts.Minimal  *)
-  (*          (fun k => exists st'', tr S!! k = Some st'' /\ j <= k /\ active_st ρ' st'') k. *)
-  (* Proof using active_st_Dec.  *)
-  (*   intros. red in EV_REL. specialize (EV_REL _ _ _ JTH HAS_LOCK PREVr). *)
-  (*   destruct EV_REL as [k EV_REL]. pattern k in EV_REL.  *)
-  (*   eapply min_prop_dec in EV_REL; eauto. *)
-  (*   intros. *)
-  (*   destruct (tr S!! n) as [st | ] eqn:NTH. *)
-  (*   2: { right. intros (? & ? & ?). congruence. } *)
-  (*   destruct (decide (j <= n)). *)
-  (*   2: { right. intros (? & ? & ?). lia. } *)
-  (*   destruct (active_st_Dec ρ' st). *)
-  (*   - left. eauto. *)
-  (*   - right. intros (? & ? & ? & ?). congruence. *)
-  (* Qed. *)
 
   Lemma eventual_release_strenghten tr ρ i (EV_REL: eventual_release tr ρ i):
     forall (ρ': R) j st' (JTH: tr S!! j = Some st')
@@ -78,17 +89,27 @@ Section FairLock.
   Definition fair_lock_progress :=
     forall (tr: mtrace EFM) (ρ: R) (i: nat) (st: St)
       (VALID: mtrace_valid tr)
-      (FROM_INIT: forall st0, tr S!! 0 = Some st0 -> is_init_st st0)
+      (FROM_INIT: forall st0, tr S!! 0 = Some st0 -> state_wf st0)
       (FAIR: inner_fair_ext_model_trace tr)
       (ITH: tr S!! i = Some st)
       (CAN_LOCK: can_lock_st ρ st)
       (ACT: active_st ρ st)
       (EV_REL: eventual_release tr ρ i),
     exists n st', i < n /\ tr S!! n = Some st' /\ has_lock_st ρ st' /\ ¬ active_st ρ st'.
+  
 
-      
+  (* TODO: mention these function equivalents of relations
+           in the definition of EM itself? *)
   Class FairLock := {
-      lock_progress: fair_lock_progress
+      lock_progress: fair_lock_progress;
+      allow_unlock_impl: fmstate M -> fmstate M;
+      allow_lock_impl: fmrole M -> fmstate M -> fmstate M;
+      allows_unlock_impl_spec st (WF: state_wf st):
+      forall st', allows_unlock st st' <-> 
+              (allow_unlock_impl st = st' /\ (exists ρ, has_lock_st ρ st /\ ¬ active_st ρ st));
+      allows_lock_impl_spec ρ st:
+      forall st', allows_lock ρ st st' <-> 
+              (allow_lock_impl ρ st = st' /\ (can_lock_st ρ st /\ ¬ active_st ρ st));
   }.
 
 End FairLock.
